### Norther theorem & Euler-Lagrangian equation

#### 1. Variation of the volume element under infinitesimal transformation

$$
det(\part_\nu \delta x^\mu)=\part_\mu \delta x^\mu
$$

The $dx^4$ transform as
$$
dx'^4 = Jdx^4
$$
where $J$ is the Jacobi determinant
$$
J=det(\frac{\part x'^\mu}{\part x^\nu})
$$
for the partial differential matrix between the old and new coordinates, a typical $J=\pm 1$ indicates the volume is not expanded or contract after the transformation. We assume a infinitesimal transformation
$$
x'^\mu=x^\mu+\delta x^\mu
$$
Then
$$
J=det(\frac{\part x'^\mu}{\part x^\nu})=det(\frac{\part x^\mu}{\part x^\nu}+\frac{\part \delta x^\mu}{\part x^\nu})=det(\delta^\mu_{~~\nu}+\part_\nu \delta x^\mu)=1+\part_\mu \delta x^\mu
$$
In the very last step, we make use of the fact that the differentiate for a determinant at $I$ is the trace (just think of identity matrix with every component added by a very small quantity, when solve for the determinant, only the linear terms at the main diagonal matter, which is the trace.ï¼‰

Therefore,
$$
dx'^4 = Jdx^4=(1+\part_\mu \delta x^\mu)dx^4
$$
And the variation of the volume element under infinitesimal transformation is
$$
\delta(dx^4)=dx'^4-dx^4=(\part_\mu \delta x^\mu) dx^4
$$

#### 2. Variation of the Lagrangian

We assume the field quantity changes at the same time that coordinates are changed, it should have a variation:
$$
\phi(x)\rightarrow\phi'(x')+\delta \phi(x)
$$
Please note that, the variation contains two part: (1) the variation of the field $\phi\rightarrow\phi'=\phi+\bar\delta \phi$ (we assume it is the same before/after the change of coordinates as is a infinitesimal transformation, for distinction we use a bar), and (2) the variation of the coordinates $x\rightarrow x'=x+\delta x$. So the field quantity has been changed, due to certain evolution of the field, while the perspective of view is also changed, such as the observer is rotated by a degree, or in a different inertial frame. The Lagrangian depends on the coordinates similarly,
$$
\delta L(x)=L'(x')-L(x)=[L'(x')-L(x')]-[L(x')-L(x)]=\bar\delta L+\part_\mu L\delta x^\mu
$$
and
$$
\bar\delta L=L'(x)-L(x)=\frac{\part L}{\part \phi}\bar\delta\phi+\frac{\part L}{\part\part_\mu\phi}\bar\delta\part_\mu\phi
$$
This is because the Lagrangian is the function of the field quantity and its 1st order differential.

 Overall, we have
$$
\delta L(x)=\frac{\part L}{\part \phi}\bar\delta\phi+\frac{\part L}{\part\part_\mu\phi}\bar\delta\part_\mu\phi+\part_\mu L\delta x^\mu
$$

#### 3. Principle of Stationary Action

Now we search for the stationary of the action by set the variation to zero:
$$
\delta S=\delta(\int d^4xL)=\int\delta(d^4x)L+\int d^4x\delta L\\
=\int d^4x(\part_\mu \delta x^\mu)L+\int d^4x(\frac{\part L}{\part \phi}\bar\delta\phi+\frac{\part L}{\part\part_\mu\phi}\bar\delta\part_\mu\phi+\part_\mu L\delta x^\mu)\\
$$
Now, we put the changes arises from coordinate transformation together, which is the first integral and the their term in the second integral:
$$
\int d^4x[(\part_\mu \delta x^\mu)L+(\part_\mu L)\delta x^\mu]+\int d^4x(\frac{\part L}{\part \phi}\bar\delta\phi+\frac{\part L}{\part\part_\mu\phi}\bar\delta\part_\mu\phi)\\
=\int d^4x \part_\mu(\delta x^\mu L)+\int d^4x (\frac{\part L}{\part \phi}\bar\delta\phi+\part_\mu(\frac{\part L}{\part\part_\mu\phi}\bar\delta\phi)-\part_\mu(\frac{\part L}{\part\part_\mu\phi})\bar\delta\phi)\\
=\int d^4x\part_\mu(L\delta x^\mu+\frac{\part L}{\part\part_\mu\phi}\bar\delta\phi)+\int d^4x\bar\delta\phi(\frac{\part L}{\part \phi}-\part_\mu\frac{\part L}{\part\part_\mu\phi})=0
$$
Now we consider:

##### (1) The coordinate is not changed:

In this case, $\delta x^\mu=0$, the first term becomes:
$$
\int d^4x\part_\mu(L\delta x^\mu+\frac{\part L}{\part\part_\mu\phi}\bar\delta\phi)=\int d^4x\part_\mu(\frac{\part L}{\part\part_\mu\phi}\bar\delta\phi)=\oint_S dS\frac{\part L}{\part\part_\mu\phi}\bar\delta\phi=0
$$
As the field quantity is fixed at the boundary of space-time, $\delta\phi=0$ in the surface integral. Now we only have the second term. At the stationary point of action, we must have:
$$
\frac{\part L}{\part \phi}-\part_\mu\frac{\part L}{\part\part_\mu\phi}=0
$$
This is literally the ==Euler-Lagrangian equation==, which governs how the field evolves through time.

##### (2)The field is not changed:

Now the variation of the field quantity with respect to certain coordinates is zero. 



